\documentclass[11pt, oneside]{article}   	% use "amsart" instead of "article" for AMSLaTeX format


% \usepackage{draftwatermark}
% \SetWatermarkText{Draft}
% \SetWatermarkScale{5}
% \SetWatermarkLightness {0.9} 
% \SetWatermarkColor[rgb]{0.7,0,0}


\usepackage{geometry}                		% See geometry.pdf to learn the layout options. There are lots.
\geometry{letterpaper}                   		% ... or a4paper or a5paper or ... 
%\geometry{landscape}                		% Activate for for rotated page geometry
%\usepackage[parfill]{parskip}    		% Activate to begin paragraphs with an empty line rather than an indent
\usepackage{graphicx}				% Use pdf, png, jpg, or epsï¿½ with pdflatex; use eps in DVI mode
								% TeX will automatically convert eps --> pdf in pdflat						
								% TeX will automatically convert eps --> pdf in pdflatex		
\usepackage{amssymb}
\usepackage{mathrsfs}
\usepackage{hyperref}
\usepackage{url}
\usepackage{subcaption}
\usepackage{authblk}
\usepackage{amsmath}
\usepackage{mathtools}
\usepackage{graphicx}
\usepackage[export]{adjustbox}
\usepackage{fixltx2e}
\usepackage{hyperref}
\usepackage{alltt}
\usepackage{color}
\usepackage[utf8]{inputenc}
\usepackage[english]{babel}
\usepackage{float}
\usepackage{bigints}
\usepackage{braket}
\usepackage{siunitx}

%
% so you can do e.g., \begin{bmatrix}[r] (or [c] or [l])
%

\makeatletter
\renewcommand*\env@matrix[1][c]{\hskip -\arraycolsep
  \let\@ifnextchar\new@ifnextchar
  \array{*\c@MaxMatrixCols #1}}
\makeatother

\newcommand{\argmax}{\operatornamewithlimits{argmax}}
\newcommand{\argmin}{\operatornamewithlimits{argmin}}

\begin{document}

\noindent
Notice that  $\sum\limits_{n = 1}^\infty (\frac{a}{b})^n  = \frac{a}{b - a}$ where $a,b \in \mathbb{N}$, $b \neq 0$ and $b - a \neq 0$. OK, but why?

\bigskip
\noindent
 Here's one way to think about it:  
      
\begin{equation*}
\begin{array}{lllll}
S
&=& \sum\limits_{n = 1}^\infty (\frac{a}{b})^n                                                                                                                &\qquad  \mathrel{\#} \text{define $S$}                                          \\ 
\vspace{2.0mm}
&=& (\frac{a}{b})^1 + (\frac{a}{b})^2 + (\frac{a}{b})^3 + \cdots                                                                                      &\qquad  \mathrel{\#} \text{expand terms}                                      \\
\vspace{2.0mm}
&\Rightarrow& (\frac{b}{a}) \cdot S = (\frac{b}{a}) \cdot [(\frac{a}{b})^1 + (\frac{a}{b})^2 + (\frac{a}{b})^3 + \cdots ]   &\qquad  \mathrel{\#} \text{multiply both sides by $\frac{b}{a}$}     \\
\vspace{2.0mm}
&\Rightarrow&  (\frac{b}{a}) \cdot S = 1 +(\frac{a}{b})^1 + (\frac{a}{b})^2 + (\frac{a}{b})^3 + \cdots                            &\qquad  \mathrel{\#} \text{multiply through on right side}              \\
\vspace{2.0mm}
&\Rightarrow&  (\frac{b}{a}) \cdot S = 1 + S                                                                                                                &\qquad  \mathrel{\#} \text{definition of $S$}                                   \\
\vspace{2.0mm}
&\Rightarrow&  (\frac{b}{a}) \cdot S - S = 1                                                                                                                 &\qquad  \mathrel{\#} \text{subtract $S$ from both sides}               \\
\vspace{2.0mm}
&\Rightarrow& \frac{bS - aS}{a} = 1                                                                                                                            &\qquad  \mathrel{\#} \text{multiply through on left side}                 \\
\vspace{2.0mm}
&\Rightarrow& S \cdot \frac{(b - a)} {a} = 1                                                                                                                 &\qquad  \mathrel{\#} \text{factor out $S$}                                       \\
\vspace{2.0mm}
&\Rightarrow& S  = \frac{a}{b - a}                                                                                                                               &\qquad  \mathrel{\#} \text{solve for $S$}
\end{array}
\end{equation*}

\bigskip
\noindent
So $S = \sum\limits_{n = 1}^\infty (\frac{a}{b})^n  =  \frac{a}{b -a}$ where $b - a \neq 0$. For example, if we  let $a =1$ and $b =2$ then \\
$\sum\limits_{n = 1}^\infty (\frac{1}{2})^n  =  \frac{1}{2-1} = 1$. Similarly, if $a =1$ and $b = 3$ then 
$\sum\limits_{n = 1}^\infty (\frac{1}{3})^n  =  \frac{1}{3-1} = \frac{1}{2}$. 

\end{document} 

